lib/Monotonic.VoidPointer.UInt32.fsti
@@ -1,10 +1,6 @@
 (**
-  * This module exposes functions to upcast from
-  * [UInt32] to [VoidPointer], and vice-versa with downcast.
-  * [upcast] ensures that the value is an upcast of [UInt32],
-  * and [downcast] ensures that the value is a downcast to
-  * [UInt32]. It also requires that the value is a valid
-  * upcast of the type.
+  * Type-safe upcasts from 32-bit integer pointers to void pointers, 
+  * and downcasts from void pointers to 32-bit integer pointers.
   *)
 
 module Monotonic.VoidPointer.UInt32
@@ -18,16 +14,15 @@ module VP = Monotonic.VoidPointer
 
 open ESPST
 
-// typedef VoidPointer_t VoidPointer_UInt32_upcast(uint32_t *p)
-
 (**
-  * `upcast` takes a pointer (buffer of length 1) to UInt32, and
-  * returns a VoidPointer in a STack effect. The function requires
-  * that the pointer is alive in memory (i.e., not a dangling pointer),
-  * and ensures that 1. the contents in memory remain unchanged, 2. the
-  * resulting VoidPointer is an upcast of the UInt32 type, and that 3.
-  * the downcasting of this VoidPointer results in the same, initial
-  * pointer to UInt32.
+  * Upcasting a 32-bit integer pointer to a void pointer. 
+  *
+  * The upcasting function requires that:
+  * - the given pointer is alive in memory;
+  * and the upcasting function ensures that:
+  * - the contents in memory remain unchanged, 
+  * - the returned void pointer is an upcast of 32-bit integer pointer, and 
+  * - downcasting the returned void pointer results in the initial integer pointer.
   *)
 val upcast (rel:G.erased (B.srel U32.t))(p: B.mpointer U32.t rel rel)
     : ESPST VP.t
@@ -38,21 +33,21 @@ val upcast (rel:G.erased (B.srel U32.t))(p: B.mpointer U32.t rel rel)
                   VP.g_downcast rel q == p /\ 
                   VP.loc_voidpointer q == B.loc_buffer p))
 
-// typedef uint32_t *VoidPointer_UInt32_downcast(VoidPointer_t p)
-
 (**
-  * `downcast` takes a VoidPointer and downcasts it back to a
-  * pointer to UInt32. Like `upcast`, `downcast` requires that
-  * the pointer is alive in memory, and ensures that the initial
-  * and final memory spaces are exactly the same, unchanged.
-  * Unlike `upcast`, it requires the VoidPointer to be an upcast
-  * of a pointer to UInt32, and ensures that the resulting pointer
-  * is, in fact, a downcast from a VoidPointer.
+  * Downcasting a void pointer to a 32-bit integer pointer.
+  *
+  * The downcasting function requires that:
+  * - the given void pointer is alive in memory, and
+  * - the given void pointer is an upcast of a 32-bit integer pointer;
+  * and the downcasting function ensures that:
+  * - the contents in memory remain unchanged, and 
+  * - upcasting the returned integer pointer results in the initial void pointer.
   *)
 val downcast (rel:G.erased (B.srel U32.t)) (p: VP.t)
     : ESPST (B.mpointer U32.t rel rel)
       (requires (fun h0 -> p `VP.is_upcast_of` rel /\ B.live h0 (VP.g_downcast rel p)))
       (ensures  (fun h0 q h1 -> 
                   h0 == h1 /\ 
+                  p `VP.is_upcast_of` rel /\
                   q == VP.g_downcast rel p /\
                   VP.loc_voidpointer p == B.loc_buffer q))
