lib/Monotonic.VoidPointer.fsti
@@ -1,6 +1,7 @@
 (**
-  * This module abstracts the tpye void* from C into a verifiable
-  * type.
+  * Interface for type-safe programming with C's void pointers based
+  * on F*'s notion of monotonic state and monotonic pointers (in which
+  * the memory is allowed to evolve only according to a given preorder).
   *)
 
 module Monotonic.VoidPointer
@@ -8,27 +9,42 @@ module Monotonic.VoidPointer
 module B = LowStar.Monotonic.Buffer
 module HS = FStar.HyperStack
 
-// typedef void* VoidPointer_t
+(**
+  * Abstract (monotonic) void pointer type.
+  *)
 val t:Type0
 
-// abstract predicate stating that the void pointer originates from upcasting an a-pointer
+(**
+  * Specifying that `p` originates from upcasting an `a`-typed monotonic 
+  * pointer, whose value is allowed to only evolve according to `rel`.
+  *)
 val is_upcast_of (p: t) (#a: Type0) (rel:B.srel a) : GTot prop
 
-// spec level "safe" downcasting of void pointers we know originate from an a-pointer
-val g_downcast (#a: Type0) (rel:B.srel a) (p: t{p `is_upcast_of` rel}) : GTot (B.mpointer a rel rel)
+(**
+  * Extracting the `a`-typed pointer from a void pointer in ghost code.
+  *)
+val g_downcast (#a: Type0) (rel:B.srel a) (p: t{p `is_upcast_of` rel}) 
+  : GTot (B.mpointer a rel rel)
 
-// when a void pointer is live in a given heap
+(**
+  * Specifying when a monotonic void pointer is live in given memory.
+  *)
 noextract
-let is_live_in (p: t) (h: HS.mem) : GTot Type0 = exists a (rel:B.srel a). p `is_upcast_of` rel /\ B.live h (g_downcast rel p)
+let is_live_in (p: t) (h: HS.mem) : GTot Type0 = 
+  exists a (rel:B.srel a). p `is_upcast_of` rel /\ B.live h (g_downcast rel p)
 
-// abstract footprint of a void pointer
+(**
+  * Abstract memory footprint of a monotonic void pointer.
+  *)
 val loc_voidpointer (p: t) : GTot B.loc
 
-// disjoint memory modifications preserve liveness of void pointers
+(**
+  * Disjoint memory modifications preserve liveness of void pointers.
+  *)
 val lemma_voidpointer_disjoint_elim (p: t) (l: B.loc) (h0 h1: HS.mem)
-: Lemma
-  (requires (B.loc_disjoint (loc_voidpointer p) l /\ p `is_live_in` h0 /\ B.modifies l h0 h1))
-  (ensures (p `is_live_in` h1))
-  [SMTPat (p `is_live_in` h0);
-   SMTPat (B.loc_disjoint (loc_voidpointer p) l);
-   SMTPat (p `is_live_in` h1)]
+  : Lemma
+    (requires (B.loc_disjoint (loc_voidpointer p) l /\ p `is_live_in` h0 /\ B.modifies l h0 h1))
+    (ensures (p `is_live_in` h1))
+    [SMTPat (p `is_live_in` h0);
+     SMTPat (B.loc_disjoint (loc_voidpointer p) l);
+     SMTPat (p `is_live_in` h1)]
