lib/VoidPointer.fst
@@ -1,6 +1,6 @@
 (**
-  * This module abstracts the tpye void* from C into a verifiable
-  * type.
+  * Instance of monotonic void pointers where the memory is allowed
+  * to evolve arbitrarily (i.e., any initial-final values are related).
   *)
 
 module VoidPointer
@@ -10,18 +10,28 @@ module VP = Monotonic.VoidPointer
 module B = LowStar.Buffer
 module HS = FStar.HyperStack
 
-// typedef void* VoidPointer_t
+(**
+  * Abstract void pointer type.
+  *)
 let t = VP.t
 
-// abstract predicate stating that the void pointer originates from upcasting an a-pointer
+(**
+  * Specifying that `p` originates from upcasting an `a`-typed pointer. 
+  *)
 let is_upcast_of p a = p `VP.is_upcast_of` (B.trivial_preorder a)
 
-// spec level "safe" downcasting of void pointers we know originate from an a-pointer
+(**
+  * Extracting the `a`-typed pointer from a void pointer in ghost code.
+  *)
 let g_downcast #a p = VP.g_downcast (B.trivial_preorder a) p
 
-// when a void pointer is live in a given heap
+(**
+  * Specifying when a void pointer is live in given memory.
+  *)
 noextract
 let is_live_in p h = VP.is_live_in p h
 
-// abstract footprint of a void pointer
+(**
+  * Abstract memory footprint of a void pointer.
+  *)
 let loc_voidpointer p = VP.loc_voidpointer p
